theories/LogicalRelation/Definition/Ell.v
@@ -9,13 +9,29 @@ Section EllRedTmEq.
     `{RedType ta} `{Typing ta} `{ConvNeuConv ta} `{ConvTerm ta}
     `{RedTerm ta} {l : TypeLevel} {Γ : context} {RNtoB : [Γ ||-S<l> arr' Γ tNat tBool] } {ℓ : ell}.
 
-  Inductive EllRedTmEq : term -> term -> Type :=
+  Inductive isLREll : term -> Type :=
+  | boxLREll {t} : [Γ ||-S< l > t : arr' Γ tNat tBool | RNtoB] ->
+    (forall n b, in_ell ℓ n b ->
+      [ Γ ||-Bool tApp t (nat_to_term n) ≅ bool_to_term b :Bool]) ->
+    isLREll (tBox ℓ t)
+  | neLREll {v} : in_ctx Γ v ℓ -> isLREll (tRel v).
+
+  Record EllRedTmEq tL tR : Type := {
+    isellL : isLREll tL;
+    isellR : isLREll tR;
+    gL : [Γ |- tL : ℓ];
+    gR : [Γ |- tR : ℓ];
+    eq : [Γ |- tL ≅ tR : ℓ];
+    eqeval : [Γ ||-S< l > tEval ℓ tL ≅ tEval ℓ tR : _ | RNtoB];
+    }.
+
+(*   Inductive EllRedTmEq : term -> term -> Type :=
   | boxReq {t t'} : [Γ ||-S< l > t ≅ t' : arr' Γ tNat tBool | RNtoB ] ->
     (forall n b, in_ell ℓ n b ->
       [ Γ ||-Bool tApp t (nat_to_term n) ≅ bool_to_term b :Bool]) ->
     EllRedTmEq (tBox ℓ t) (tBox ℓ t')
   | neRed {v} : in_ctx Γ v ℓ -> EllRedTmEq (tRel v) (tRel v).
-
+ *)
 (*   Section Def.
     Context `{!GenericTypingProperties _ _ _ _ _ _ _ _ _}.
 
@@ -36,6 +52,8 @@ End EllRedTmEq.
 Export EllRedTmEq(EllRedTmEq).
 Notation "[ Γ ||-EllS t ≅ u : ℓ | RNtoB ]" := (EllRedTmEq Γ RNtoB ℓ t u) 
   (at level 0, Γ, t, u, ℓ, RNtoB at level 50).
+Notation "[ Γ ||-EllS t : ℓ | RNtoB ]" := (EllRedTmEq Γ RNtoB ℓ t t) 
+  (at level 0, Γ, t, ℓ, RNtoB at level 50).
 
 Section WEllRedTmEq.
   Context `{ta : tag} `{WfContext ta} `{WfType ta} `{ConvType ta}
@@ -45,8 +63,10 @@ Section WEllRedTmEq.
     dSplit (fun Δ _ (ρ: Δ ≤ Γ) hSplit => [ Δ ||-EllS t⟨ρ⟩ ≅ u⟨ρ⟩ : ℓ | hSplit]) RNtoB.
 End WEllRedTmEq.
 
-Notation "[ Γ ||-Ell t ≅ u : ℓ | RNtoB ]" := (WEllRedTmEq Γ RNtoB ℓ t u) 
+Notation "[ Γ ||-Ell t ≅ u : ℓ | RNtoB ]" := (WEllRedTmEq Γ RNtoB ℓ t u)
   (at level 0, Γ, t, u, ℓ, RNtoB at level 50).
+Notation "[ Γ ||-Ell t : ℓ | RNtoB ]" := (WEllRedTmEq Γ RNtoB ℓ t t)
+  (at level 0, Γ, t, ℓ, RNtoB at level 50).
 
 
 
