theories/LogicalRelation/Introductions/Pi.v
@@ -17,22 +17,40 @@ Section PolyRedPi.
     [Γ ||-S<l> tProd A B ≅ tProd A' B'] :=
     LRPi' (LRPiPoly0 wfΓ PAB).
 
+  Definition Build_PiRedTmEq' {Γ l A B} {ΠA : PiRedTy Γ l A B} {t u : term}
+    (shp := PiRedTy.domL ΠA) (shp' := PiRedTy.domR ΠA)
+    (pos := PiRedTy.codL ΠA) (pos' := PiRedTy.codR ΠA)
+    (redL : PiRedTm ΠA t) (redR : PiRedTm ΠA u)
+    (nfL := PiRedTmEq.nf redL) (nfR := PiRedTmEq.nf redR) :
+    [Γ |- nfL ≅ nfR : tProd shp pos] ->
+    (forall Δ ρ wfΔ a b
+      (hab : [Δ ||-S< l > a ≅ b : shp⟨ρ⟩ | PolyRed.shpRed ΠA ρ wfΔ ]), 
+      [Δ ||-< l > tApp nfL⟨ρ⟩ a ≅ tApp nfR⟨ρ⟩ b : pos⟨wk_up shp ρ⟩[a ..]
+        | PolyRed.posRed ΠA ρ wfΔ hab]) ->
+    [Γ ||-Π t ≅ u : A | ΠA].
+  Proof.
+    intros eq eqApp.
+    econstructor.
+    1: eapply eq.
+    intros Δ a b ρ wfΔ hab.
+    eapply eqApp.
+  Qed.
+
+
+
+  Lemma canonPi `{GenericTypingProperties} {Γ A A' B B' l p p'}
+    {RΠ : [Γ ||-S< l > tProd A B ≅ tProd A' B']} :
+    [ Γ ||-S< l > p ≅ p' : tProd A B | RΠ] ->
+    [ Γ ||-S< l > p ≅ p' : tProd A B | LRPi' (normRedΠ RΠ)].
+  Proof.
+    intro. now eapply SirrLR.
+  Qed.
+
+  Lemma canonPi_inv `{GenericTypingProperties} {Γ A A' B B' l p p'}
+    {RΠ : [Γ ||-S< l > tProd A B ≅ tProd A' B']} :
+    [ Γ ||-S< l > p ≅ p' : tProd A B | LRPi' (normRedΠ RΠ)] ->
+    [ Γ ||-S< l > p ≅ p' : tProd A B | RΠ].
+  Proof.
+    intro. now eapply SirrLR.
+  Qed.
 End PolyRedPi.
-
-
-
-Lemma canonPi `{GenericTypingProperties} {Γ A A' B B' l p p'}
-  {RΠ : [Γ ||-S< l > tProd A B ≅ tProd A' B']} :
-  [ Γ ||-S< l > p ≅ p' : tProd A B | RΠ] ->
-  [ Γ ||-S< l > p ≅ p' : tProd A B | LRPi' (normRedΠ RΠ)].
-Proof.
-  intro. now eapply SirrLR.
-Qed.
-
-Lemma canonPi_inv `{GenericTypingProperties} {Γ A A' B B' l p p'}
-  {RΠ : [Γ ||-S< l > tProd A B ≅ tProd A' B']} :
-  [ Γ ||-S< l > p ≅ p' : tProd A B | LRPi' (normRedΠ RΠ)] ->
-  [ Γ ||-S< l > p ≅ p' : tProd A B | RΠ].
-Proof.
-  intro. now eapply SirrLR.
-Qed.
