theories/LogicalRelation/Introductions/Ell.v
@@ -11,6 +11,8 @@ Section Ell.
     + intros. eapply SnatRed; tea.
     + intros. eapply SboolRed; tea.
   Qed.
+  Lemma NtoBRedEqTy {Γ : context} (wfΓ : [|-Γ]) {l} : [Γ ||-< l > arr' Γ tNat tBool ].
+  Proof. now eapply WAd_return, SNtoBRedEqTy. Qed.
 
 
   Lemma EvalRelRedEqAux {ℓ : ell} {Γ l v} (wfΓ : [|-Γ]) : in_ctx Γ v ℓ -> (forall tL tR (Rt : [Γ ||-Nat tL ≅ tR :Nat]), forall k,
@@ -49,6 +51,7 @@ Section Ell.
   Qed.
 
 
+
   Lemma EvalRelRedEq {ℓ : ell} {Γ l v t t' k} (wfΓ :[|-Γ]):  in_ctx Γ v ℓ -> [Γ ||-S< l > t ≅ t' : tNat | SnatRed (l:=l) wfΓ ] ->
     [ Γ ||-S< l > tApp (tEval ℓ (tRel v)) (nSucc k t) ≅ tApp (tEval ℓ (tRel v)) (nSucc k t') : tBool |SboolRed wfΓ].
   Proof.
@@ -58,50 +61,747 @@ Section Ell.
     Unshelve. tea.
   Qed.
 
-  Lemma EvalRedEq {Γ l t t'} {ℓ : ell} (wfΓ : [|-Γ]) (RNtoB : [Γ ||-S<l> arr' Γ tNat tBool])
+  Lemma EvalRedEq {Γ l t t'} {ℓ : ell} (RNtoB : [Γ ||-S<l> arr' Γ tNat tBool])
      : [ Γ ||-EllS t ≅ t' : ℓ | RNtoB ] -> [ Γ ||-S< l > tEval ℓ t ≅ tEval ℓ t' : _ | RNtoB].
   Proof.
-    intros Rtt'.
-    destruct Rtt' as [?? Rtt' Rconv|].
-    + escape.
-      eapply SredSubstTmEq; tea.
-      all: eapply redtm_evalBox; tea.
-      all: intros n b inℓ; specialize (Rconv n b inℓ).
-      2: etransitivity.
-      1,3 : eapply (escapeTm (SboolRed _)); tea.
-      symmetry.
-      eapply (escapeSplitTm (boolRed ltac:(tea))).
-      eapply (appcongTerm _ (Wpack_return Rtt')).
-      unshelve eapply Wpack_return, nat_to_termReq; tea.
-      eapply natRedTy; tea.
-    + eapply canonPi_inv. cbn.
-      assert [ |- Γ ,, tNat] by (eapply wfc_cons; gtyping).
-      assert [Γ,,tNat |- tBool] as HB by
-        (eapply wft_term, ty_bool; tea).
-      assert [Γ |-[ ta ] tProd tNat tBool ≅ arr' Γ tNat tBool] as Harr by
-        (eapply convty_term, convtm_prod, convtm_bool; tea; gtyping).
-      unshelve econstructor.
-      1,2 :  econstructor; cbn; [ eapply redtmwf_refl, ty_eval, ty_var; tea
-        |eapply EvalLRFun; cbn; tea].
-      - cbn. eapply convtm_eta, convtm_convneu, (convneu_eval (k:=0)),
-          convneu_var; tea.
-        2,4: eapply ty_eval, ty_var; tea.
-        1:gtyping.
-        1,2: constructor; tea.
-        1: constructor. Search _wk_id.
-        1: cbn; rewrite wk_to_ren_id;
-          now eapply in_there with (A:=ℓ).
-        1: eapply (ty_var0 (A:=tNat)); gtyping.
-      - cbn[PiRedTmEq.nf]. unfold PiRedTmEq.appRed.
-        intros ???? wfΔ ?.
-        eapply Split_return; tea.
-        intros Ξ wfΞ ρΞ oRΠ.
-        unshelve eapply SirrLR, SwkLR.
-        3: eapply SboolRed; tea.
-        all:tea. cbn.
-        unshelve eapply (EvalRelRedEq (k:=0)), SirrLR, hab; tea.
-        eapply in_ctx_wk with (d:=ℓ); tea.
-        Unshelve. all: tea.
+    assert (wfΓ : [|-Γ]) by (escape; gtyping).
+    intros Rtt'. eapply Rtt'.
   Qed.
 
+  Lemma symmetricEll{Γ l n n' ℓ} (RNtoB : [Γ ||-S< l > arr' Γ tNat tBool]) :
+    [Γ ||-EllS n ≅ n' : ℓ | RNtoB] -> [Γ ||-EllS n' ≅ n : ℓ | RNtoB].
+  Proof.
+    intros [].
+    constructor; tea; symmetry; tea.
+  Qed.
+
+  Lemma transitiveEll {Γ l n n' n'' ℓ} (RNtoB : [Γ ||-S< l > arr' Γ tNat tBool]) :
+    [Γ ||-EllS n ≅ n' : ℓ | RNtoB] -> [Γ ||-EllS n' ≅ n'' : ℓ | RNtoB] -> [Γ ||-EllS n ≅ n'' : ℓ | RNtoB].
+  Proof.
+    intros [] [].
+    constructor; tea; etransitivity; tea.
+  Qed.
+
+  Instance PER_Ell l Γ RNtoB ℓ : PER (EllRedTmEq (l:=l) Γ RNtoB ℓ).
+  Proof.
+    constructor.
+    + intros n n'. eapply symmetricEll.
+    + intros n n' n''. eapply transitiveEll.
+  Qed.
+
+  Lemma SirrEll {Γ l t t'} {ℓ : ell} (RNtoB RNtoB' : [Γ ||-S< l > arr' Γ tNat tBool]) :
+    [Γ ||-EllS t ≅ t' : ℓ | RNtoB] -> [Γ ||-EllS t ≅ t' : ℓ | RNtoB'].
+  Proof.
+    intros Rtt'.
+    destruct Rtt' eqn:eRtt'.
+    constructor; tea.
+    + destruct isellL; constructor; tea.
+      eapply SirrLR; tea.
+    + destruct isellR; constructor; tea.
+      eapply SirrLR; tea.
+    + eapply SirrLR; tea.
+  Qed.
+
+  Lemma wkisell {Γ Δ l t}  {ℓ : ell} (ρ : Δ ≤ Γ) (wfΔ : [|-Δ]) (RNtoB : [Γ ||-S< l > arr' Γ tNat tBool]) :
+    EllRedTmEq.isLREll (RNtoB:=RNtoB) (ℓ:=ℓ) t -> EllRedTmEq.isLREll (RNtoB:=wkRed (SwkLR _ _ _ RNtoB) ρ wfΔ) (ℓ:=ℓ) t⟨ρ⟩.
+  Proof.
+    assert (wfΓ : [|-Γ]) by (escape; gtyping).
+    intros isellt.
+    destruct isellt as [t' Rt Rtnb|]; rewrite <-? wk_box; constructor; tea.
+    - unshelve (eapply SirrLR, SwkLR; tea); tea.
+    - change [?Γ ||-Bool ?tL ≅ ?tR :Bool] with [Γ ||-S< l > tL ≅ tR :_ | SboolRed wfΔ].
+      change [?Γ ||-Bool ?tL ≅ ?tR :Bool] with [Γ ||-S< l > tL ≅ tR :_ | SboolRed wfΓ] in Rtnb.
+      intros n b inℓ.
+      rewrite <- (wk_nat_to_term ρ), <- (wk_bool_to_term ρ), wk_app.
+      now unshelve now eapply SirrLREq, SwkLR, Rtnb.
+    - eapply in_ctx_wk with (d:=ℓ); tea.
+  Qed.
+  Lemma SwkEll {Γ Δ l t t'} {ℓ : ell} (ρ : Δ ≤ Γ) (wfΔ : [|-Δ]) (RNtoB : [Γ ||-S< l > arr' Γ tNat tBool]) :
+    [Γ ||-EllS t ≅ t' : ℓ | RNtoB] -> [Δ ||-EllS t⟨ρ⟩ ≅ t'⟨ρ⟩ : ℓ | wkRed (SwkLR _ _ _ RNtoB) ρ wfΔ].
+  Proof.
+    assert (wfΓ : [|-Γ]) by (escape; gtyping).
+    intros [].
+    constructor.
+    1,2: refine (wkisell _ _ _ _); tea.
+    1,2: eapply (ty_wk (A:=ℓ)); tea.
+    1: eapply (convtm_wk (A:=ℓ)); tea.
+    rewrite ! wk_eval.
+    unshelve eapply SirrLR, SwkLR, eqeval; tea.
+  Qed.
+
+  Lemma WEll_return {Γ l t t'} {ℓ : ell} (RNtoB : [Γ ||-S< l > arr' Γ tNat tBool])
+    (WRNtoB : [Γ ||-< l > arr' Γ tNat tBool]) :
+    [Γ ||-EllS t ≅ t' : ℓ | RNtoB] -> [Γ ||-Ell t ≅ t' : ℓ | WRNtoB].
+  Proof.
+    assert (wfΓ : [|-Γ]) by (escape; gtyping).
+    intros Rt.
+    eapply Split_return; tea.
+    intros ??? oRNtoB.
+    unshelve eapply SirrEll, SwkEll; tea.
+  Qed.
+
+
+  Lemma isLREll_isWfEll {Γ l ℓ t} (RNtoB : [Γ ||-S< l > arr' Γ tNat tBool]):
+    EllRedTmEq.isLREll (Γ:=Γ) (RNtoB:=RNtoB) (ℓ:=ℓ) (l:=l) t -> isWfEll Γ ℓ t.
+  Proof.
+    intros isellt.
+    assert (wfΓ :[|-Γ]) by (escape; gtyping).
+    destruct isellt as [t Rt Rtnb|]; constructor; tea.
+    + escape; tea.
+    + intros n b inℓ.
+      eapply escapeTm.
+      change [?Γ ||-Bool ?tL ≅ ?tR :Bool]
+        with [Γ ||-S< l > tL ≅ tR :_ | SboolRed wfΓ] in *.
+      now eapply Rtnb.
+  Qed.
+
+  Lemma escapeEll {Γ l n n' ℓ} (RNtoB : [Γ ||-S< l > arr' Γ tNat tBool]) : [Γ ||-EllS n ≅ n' : ℓ | RNtoB] -> [Γ |- n : ℓ] × [Γ |- n' : ℓ] × [Γ |- n ≅ n' : ℓ].
+  Proof.
+    assert (wfΓ : [|-Γ]) by (escape; gtyping).
+    intros [].
+    prod_splitter; tea.
+  Qed.
+
+  Lemma SreflectEll {Γ l} {ℓ : ell} {v} (RNtoB : [Γ ||-S< l > arr' Γ tNat tBool]) :
+    in_ctx Γ v ℓ -> [Γ ||-EllS tRel v : ℓ | RNtoB].
+  Proof.
+    assert (wfΓ : [|-Γ]) by (escape; gtyping).
+    intros inΓ.
+    constructor.
+    1,2: constructor; tea.
+    1,2: eapply ty_var; tea.
+    1: eapply convtm_varEll; tea.
+    assert [ |- Γ ,, tNat] as wfΓN by (eapply wfc_cons; gtyping).
+    assert [Γ,,tNat |- tBool] as gB by
+      (eapply wft_term, ty_bool; tea).
+    assert [Γ |-[ ta ] arr' Γ tNat tBool ≅ arr' Γ tNat tBool] as gNtoB by
+      (eapply convty_term, convtm_prod, convtm_bool; tea; gtyping).
+    eapply canonPi_inv.
+    unshelve eapply Build_PiRedTmEq'.
+    1,2: econstructor; cbn ; [eapply redtmwf_refl, ty_eval, ty_var; tea
+      | eapply EvalLRFun; cbn; tea].
+    - cbn. eapply convtm_eta, convtm_convneu, (convneu_eval (k:=0)),
+        convneu_var; tea.
+      2,4: eapply ty_eval, ty_var; tea.
+      1:gtyping.
+      1,2: constructor; tea.
+      1: constructor.
+      1: cbn; rewrite wk_to_ren_id;
+        now eapply in_there with (A:=ℓ).
+      1: eapply (ty_var0 (A:=tNat)); gtyping.
+    - cbn[PiRedTmEq.nf].
+      intros *.
+      unshelve eapply Wpack_return'.
+      1: unshelve eapply SboolRed; tea.
+      eapply (EvalRelRedEq (k:=0)), SirrLR, hab.
+      eapply in_ctx_wk with (d:=ℓ); tea.
+  Qed.
+  Lemma Svar0Ell {Γ l} {ℓ : ell} (RNtoB : [Γ,,ℓ ||-S< l > arr' Γ tNat tBool]) : [Γ,,ℓ ||-EllS tRel 0 : ℓ | RNtoB].
+  Proof.
+    eapply SreflectEll.
+    constructor.
+  Qed.
+  Lemma reflectEll {Γ l} {ℓ : ell} {v} (RNtoB : [Γ ||-< l > arr' Γ tNat tBool]) :
+    in_ctx Γ v ℓ -> [Γ ||-Ell tRel v : ℓ | RNtoB].
+  Proof.
+    assert (wfΓ : [|-Γ]) by (escape; gtyping).
+    intros inℓ.
+    unshelve now eapply WEll_return, SreflectEll.
+    now eapply SNtoBRedEqTy.
+  Qed.
+  Lemma var0Ell {Γ l} {ℓ : ell} (RNtoB : [Γ,,ℓ ||-< l > arr' Γ tNat tBool]) : [Γ,,ℓ ||-Ell tRel 0 : ℓ | RNtoB].
+  Proof.
+    eapply reflectEll.
+    constructor.
+  Qed.
+
+  Lemma SboxRed {Γ l t t'} {ℓ : ell} (RNtoB : [Γ ||-S<l> arr' Γ tNat tBool]) :
+    [Γ ||-S< l > t ≅ t' : _ | RNtoB] ->
+    (forall n b, in_ell ℓ n b ->
+      [Γ ||-Bool tApp t (nat_to_term n) ≅ bool_to_term b :Bool]) ->
+    (forall n b, in_ell ℓ n b ->
+      [Γ ||-Bool tApp t' (nat_to_term n) ≅ bool_to_term b :Bool]) ->
+    [Γ ||-EllS tBox ℓ t ≅ tBox ℓ t' : ℓ | RNtoB].
+  Proof.
+    assert (wfΓ :[|-Γ]) by (escape; gtyping).
+    intros Rtt' Btnb Bt'nb.
+    escape.
+    constructor.
+    1,2: constructor.
+    1: eapply lrefl; tea.
+    2: eapply urefl; tea.
+    3,4: eapply ty_box; tea.
+    5: eapply convtm_box; tea.
+    6: eapply SredSubstTmEq; tea; eapply redtm_evalBox; tea.
+    1-7: intros n b inℓ.
+    3-7: unshelve eapply (escapeTm (SboolRed wfΓ)); tea; cbn.
+    1-7: eauto.
+  Qed.
+
+  Lemma dSplit_bind_ell {Γ} (wfΓ : [|-Γ]) {A} {ℓ : ell} {P : nat -> bool -> Monad.dPSh Γ A}
+    {hA : Split A} (hP : forall n b, in_ell ℓ n b -> dSplit (P n b) hA) :
+    dSplit (fun Δ wfΔ ρ hA => forall n b, in_ell ℓ n b -> P n b Δ wfΔ ρ hA) hA.
+  Proof.
+    induction ℓ as [| ℓ n b ihℓ] using ell_rect .
+    + eapply Split_return; tea.
+      intros ?????? [].
+    + assert (hP' : forall n b, in_ell ℓ n b -> dSplit (P n b) hA).
+      { intros n' b' inℓ'.
+        eapply hP. eapply in_cons_ell. now right. }
+      specialize (ihℓ hP'); clear hP'.
+      specialize (hP n b ltac:(eapply in_cons_ell; left; repeat constructor)).
+      eapply (dSplit_bind hP).
+      intros ??? ohA ohP.
+      unshelve eapply (dSplit_wk_bind_return ihℓ); tea.
+      intros ??? _ oihℓ ohA' n' b' [[-> ->]| [inℓ]]%in_cons_ell_relevant.
+      - now eapply hP, overtree_PSh.
+      - eapply ihℓ; tea.
+  Qed.
+
+  Lemma boxRed {Γ l t t'} {ℓ : ell} (wfΓ : [|-Γ]) :
+    [Γ ||-< l > t ≅ t' : _ | NtoBRedEqTy (l:=l) wfΓ] ->
+    (forall n b, in_ell ℓ n b ->
+      [Γ ||-< l > tApp t (nat_to_term n) ≅ bool_to_term b : _ | boolRed (l:=l) wfΓ]) ->
+    [Γ ||-Ell tBox ℓ t ≅ tBox ℓ t' : ℓ | NtoBRedEqTy (l:=l) wfΓ].
+  Proof.
+    intros Rtt' Rtnb.
+    assert (Rt'nb : forall n b, in_ell ℓ n b ->
+      [Γ ||-< l > tApp t' (nat_to_term n) ≅ bool_to_term b : _ | boolRed (l:=l) wfΓ]).
+    { intros ?? inℓ.
+      specialize (Rtnb _ _ inℓ).
+      etransitivity; tea.
+      symmetry.
+      eapply simple_appcongTerm; tea.
+      now unshelve eapply nat_to_termReq. }
+    eapply dSplit_bind_ell in Rtnb; tea.
+    eapply dSplit_bind_ell in Rt'nb; tea.
+    eapply (dSplit_bind Rtt'). Unshelve.
+    intros Δ wfΔ ρ _ oRtt'.
+    unshelve eapply (dSplit_wk_bind Rtnb); tea.
+    intros Ξ wfΞ ρΞ _ oRtnb.
+    unshelve eapply (dSplit_wk_bind_return Rt'nb); tea.
+    { eapply wk_well_wk_compose; tea. }
+    intros Ω wfΩ ρΩ obool oRt'nb oNtoR.
+    rewrite <-! wk_box.
+    eapply SboxRed.
+    - now eapply Rtt', overtree_PSh.
+    - change [?Γ ||-Bool ?tL ≅ ?tR :Bool] with
+        [Γ ||-S< l > tL ≅ tR :_ | SboolRed wfΩ] in *.
+      intros n b inℓ.
+      rewrite <- (wk_nat_to_term ((ρΩ ∘w ρΞ) ∘w ρ)),
+        <- (wk_bool_to_term ((ρΩ ∘w ρΞ) ∘w ρ)).
+      unshelve eapply SirrLR, Rtnb; tea.
+      all: rewrite wk_comp_assoc; tea.
+      now eapply overtree_PSh.
+    - change [?Γ ||-Bool ?tL ≅ ?tR :Bool] with
+        [Γ ||-S< l > tL ≅ tR :_ | SboolRed wfΩ] in *.
+      intros n b inℓ.
+      rewrite <- (wk_nat_to_term ((ρΩ ∘w ρΞ) ∘w ρ)),
+        <- (wk_bool_to_term ((ρΩ ∘w ρΞ) ∘w ρ)).
+      unshelve eapply SirrLR, Rt'nb; tea.
+      all: now rewrite wk_comp_assoc.
+  Qed.
+
+Ltac escape :=
+  repeat lazymatch goal with
+  | [H : [_ ||-S< _ > _] |-  _ ] =>
+    try
+     (let Xl := fresh "EscL" H in
+      let Xr := fresh "EscR" H in
+      let X := fresh "Esc" H in
+      pose proof (escapeTy H) as (Xl & Xr & X) );
+    block H
+  | [H : [_ ||-S<_> _ ≅ _  : _ | ?RA ] |- _] =>
+    try
+     (let Xl := fresh "EscL" H in
+      let Xr := fresh "EscR" H in
+      let X := fresh "Esc" H in
+      pose proof (escapeTm RA H) as (Xl & Xr & X) );
+      block H
+  | [H : [_ ||-< _ > _] |-  _ ] =>
+    try
+     (let Xl := fresh "EscL" H in
+      let Xr := fresh "EscR" H in
+      let X := fresh "Esc" H in
+      pose proof (escapeSplitTy H) as (Xl & Xr & X) );
+    block H
+  | [H : [_ ||-<_> _ ≅ _  : _ | ?RA ] |- _] =>
+    try
+     (let Xl := fresh "EscL" H in
+      let Xr := fresh "EscR" H in
+      let X := fresh "Esc" H in
+      pose proof (escapeSplitTm _ H) as (Xl & Xr & X) );
+      block H
+  | [H : [_ ||-EllS _ ≅ _ : _ | _] |- _] =>
+    try
+      (let Xl := fresh "EscL" H in
+      let Xr := fresh "EscR" H in
+      let X := fresh "Esc" H in
+      pose proof (escapeEll _ H) as (Xl & Xr & X) );
+      block H
+  end; unblock.
+
+
+  Lemma evalnat_to_termRed {Γ l n n' k b} {ℓ : ell} (wfΓ : [|-Γ]) : in_ell ℓ k b -> [Γ ||-EllS n ≅ n' : ℓ | SNtoBRedEqTy (l:=l) wfΓ] ->
+    [Γ ||-S< l > tApp (tEval ℓ n) (nat_to_term k) ≅ bool_to_term b : _ | SboolRed wfΓ].
+  Proof.
+    intros inℓ Rnn'.
+    destruct Rnn' as [[t Rt Rtb|] elln' gn gn' geqnn' Reval].
+    - eapply SredSubstLeftTmEq.
+      2: eapply (redtm_app (B:=tBool)), ty_nSucc, ty_zero; tea.
+      2: eapply redtm_evalBox; tea.
+      2: escape; tea.
+      2: clear n b inℓ; intros n b inℓ;
+        unshelve eapply (escapeTm (SboolRed wfΓ)), Rtb; tea.
+      eapply Rtb; tea.
+    - eapply SredSubstLeftTmEq, redtm_evalRel; tea.
+      eapply Sbool_to_termRed.
+  Qed.
+
+  Lemma Evalnat_to_term {ℓ : ell} {Γ l t n b} (RNtoB : [Γ ||-S< l > arr' Γ tNat tBool]) : in_ell ℓ n b ->
+    [Γ ||-EllS t : ℓ |RNtoB] -> [Γ ||-Bool tApp (tEval ℓ t) (nat_to_term n) ≅ bool_to_term b :Bool].
+  Proof.
+    intros inℓ Rt.
+    assert (wfΓ : [|-Γ]) by (escape; gtyping).
+    eapply evalnat_to_termRed with (wfΓ:=wfΓ); tea.
+    now eapply SirrEll.
+  Qed.
+
+  Lemma evalBoxRed {Γ l t} {ℓ : ell} (RNtoB : [Γ ||-S< l > arr' Γ tNat tBool]) :
+    (forall n b, in_ell ℓ n b -> [Γ ||-Bool tApp t (nat_to_term n) ≅ bool_to_term b :Bool]) ->
+    [Γ ||-S< l > t :_ | RNtoB] -> [Γ ||-S< l > tEval ℓ (tBox ℓ t) ≅ t : _ | RNtoB].
+  Proof.
+    intros Rtnb Rt.
+    assert (wfΓ : [|-Γ]) by (escape; gtyping).
+    change [?Γ ||-Bool ?tL ≅ ?tR :Bool] with
+      [Γ ||-S< l > tL ≅ tR :_ | SboolRed wfΓ] in *.
+    eapply SredSubstLeftTmEq, redtm_evalBox; tea.
+    2: intros n b inℓ; specialize (Rtnb _ _ inℓ).
+    all: escape; tea.
+  Qed.
+
+  Lemma SboxEvalRedEq {Γ l ℓ t t'} (RNtoB : [Γ ||-S< l > arr' Γ tNat tBool]) :
+    [Γ ||-EllS t ≅ t' : ℓ | RNtoB] -> [Γ ||-EllS tBox ℓ (tEval ℓ t) ≅ tBox ℓ (tEval ℓ t') : ℓ |RNtoB].
+  Proof.
+    intros Rt.
+    eapply SboxRed.
+    { eapply Rt. }
+    1,2: intros; eapply Evalnat_to_term; tea.
+    + eapply lrefl; tea.
+    + eapply urefl; tea.
+  Qed.
+
+  Lemma etaEllRed {Γ l ℓ t} (RNtoB : [Γ ||-S< l > arr' Γ tNat tBool]) :
+    [Γ ||-EllS t : ℓ | RNtoB] -> [Γ ||-EllS tBox ℓ (tEval ℓ t) ≅ t : ℓ |RNtoB].
+  Proof.
+    intros Rt.
+    assert (wfΓ : [|-Γ]) by (escape; gtyping).
+    destruct Rt eqn:eRt.
+    constructor; tea.
+    + constructor; tea.
+      intros n b inℓ; eapply Evalnat_to_term, lrefl; tea.
+    + eapply escapeEll.
+      eapply SboxEvalRedEq; tea.
+    + escape.
+      eapply convtm_eta_ell; tea.
+      - eapply escapeEll.
+        eapply SboxEvalRedEq; tea.
+      - constructor; tea.
+        intros n b inℓ.
+        eapply escapeTm, @evalnat_to_termRed with (wfΓ := wfΓ); tea.
+        eapply SirrEll; tea.
+      - now eapply isLREll_isWfEll.
+      - eapply escapeTm, evalBoxRed, Rt.
+        intros n b inℓ.
+        eapply evalnat_to_termRed with (wfΓ:=wfΓ); tea.
+        now eapply SirrEll.
+    + eapply evalBoxRed, Rt.
+      intros n b inℓ.
+      eapply evalnat_to_termRed with (wfΓ:=wfΓ); tea.
+      now eapply SirrEll.
+  Qed.
+
+
+  Section SEllElimRedEq.
+  Context {Γ l ℓ k P P' t t' b b'} (wfΓ : [|-Γ]) (ℓt := cons_ell ℓ k true) (ℓf := cons_ell ℓ k false)
+    (RB := SboolRed (l:=l) wfΓ) (RN := SnatRed (l:=l) wfΓ)
+    (RNtoB := SNtoBRedEqTy (l:=l) wfΓ)
+    (gP : [Γ,,ℓ |- P]) (gP' : [Γ,,ℓ |- P']) (gPP' : [Γ,,ℓ |- P ≅ P'])
+    (RPP'ext : forall Δ (ρ : Δ ≤ Γ) (wfΔ : [|-Δ]), forall t t', [Δ ||-EllS t ≅ t' : ℓ | SNtoBRedEqTy (l:=l) wfΔ] ->
+      [Δ ||-< l > P⟨wk_up ℓ ρ⟩[t..] ≅ P'⟨wk_up ℓ ρ⟩[t'..]])
+    (Rt  : [Γ ||-EllS t ≅ t' : ℓ | RNtoB]) (Rb : [Γ ||-S< l > b ≅ b' : tBool | RB])
+    (Rtkb : [Γ ||-S< l > tApp (tEval ℓ t) (nat_to_term k) ≅ b : tBool | RB])
+    (Rt'kb : [Γ ||-S< l > tApp (tEval ℓ t') (nat_to_term k) ≅ b : tBool | RB])
+    (Pt := P⟨wk_up ℓ (@wk1 Γ ℓt)⟩[(tBox ℓ (tEval ℓt (tRel 0)))..])
+    (Pf := P⟨wk_up ℓ (@wk1 Γ ℓf)⟩[(tBox ℓ (tEval ℓf (tRel 0)))..])
+    (P't := P'⟨wk_up ℓ (@wk1 Γ ℓt)⟩[(tBox ℓ (tEval ℓt (tRel 0)))..])
+    (P'f := P'⟨wk_up ℓ (@wk1 Γ ℓf)⟩[(tBox ℓ (tEval ℓf (tRel 0)))..])
+    (wfΓℓ := wfc_consell (ℓ:=ℓ) wfΓ)
+    (wfΓℓt := wfc_consell (ℓ:=ℓt) wfΓ)
+    (wfΓℓf := wfc_consell (ℓ:=ℓf) wfΓ).
+  Let RPP' : [Γ,,ℓ ||-< l > P ≅ P'].
+  Proof.
+    rewrite <- (wk1_eta (Γ:=Γ) (A:=ℓ) (t:=P)), <- (wk1_eta (Γ:=Γ) (A:=ℓ) (t:=P')).
+    unshelve eapply RPP'ext; tea.
+    eapply SreflectEll.
+    repeat constructor.
+  Qed.
+  Let RPP'extt : forall Δ (ρ : Δ ≤ Γ) (wfΔ : [|-Δ]), forall n n', [Δ ||-EllS n ≅ n' : ℓt | SNtoBRedEqTy (l:=l) wfΔ] ->
+      [Δ ||-< l > P⟨wk_up ℓ ρ⟩[(tBox ℓ (tEval ℓt n))..] ≅ P'⟨wk_up ℓ ρ⟩[(tBox ℓ (tEval ℓt n'))..]].
+  Proof.
+    intros * Rn0.
+    unshelve eapply RPP'ext; tea.
+    eapply SboxRed.
+    + eapply EvalRedEq; tea.
+    + intros ?? inℓ.
+      eapply evalnat_to_termRed; tea.
+      eapply in_cons_ell; right; tea.
+    + intros ?? inℓ.
+      eapply evalnat_to_termRed, PER_Symmetric; tea.
+      eapply in_cons_ell; right; tea.
+  Qed.
+  Let RPP'extf : forall Δ (ρ : Δ ≤ Γ) (wfΔ : [|-Δ]), forall n n', [Δ ||-EllS n ≅ n' : ℓf | SNtoBRedEqTy (l:=l) wfΔ] ->
+      [Δ ||-< l > P⟨wk_up ℓ ρ⟩[(tBox ℓ (tEval ℓf n))..] ≅ P'⟨wk_up ℓ ρ⟩[(tBox ℓ (tEval ℓf n'))..]].
+  Proof.
+    intros * Rn0.
+    unshelve eapply RPP'ext; tea.
+    eapply SboxRed.
+    + eapply EvalRedEq; tea.
+    + intros ?? inℓ.
+      eapply evalnat_to_termRed; tea.
+      eapply in_cons_ell; right; tea.
+    + intros ?? inℓ.
+      eapply evalnat_to_termRed, PER_Symmetric; tea.
+      eapply in_cons_ell; right; tea.
+  Qed.
+
+  Let RPP't : [Γ ||-< l > P[t..] ≅ P'[t'..]].
+  Proof.
+    rewrite <- (wk_id_ren_on (Γ,,ℓ) P), <- (wk_id_ren_on (Γ,,ℓ) P'),
+      <- 2 wk_up_wk_id.
+    unshelve eapply RPP'ext; tea.
+  Qed.
+  Context {ht ht' hf hf'}
+    (Rhtext : forall Δ (ρ : Δ ≤ Γ) (wfΔ : [|-Δ]), forall n n' (Rn : [Δ ||-EllS n ≅ n' : ℓt | SNtoBRedEqTy (l:=l) wfΔ]),
+      [Δ ||-< l > ht⟨wk_up ℓt ρ⟩[n..] ≅ ht'⟨wk_up ℓt ρ⟩[n'..] : P⟨wk_up ℓ ρ⟩[(tBox ℓ (tEval ℓt n))..] | RPP'extt Δ ρ wfΔ _ _ Rn])
+    (Rhfext : forall Δ (ρ : Δ ≤ Γ) (wfΔ : [|-Δ]), forall n n' (Rn : [Δ ||-EllS n ≅ n' : ℓf | SNtoBRedEqTy (l:=l) wfΔ]),
+      [Δ ||-< l > hf⟨wk_up ℓf ρ⟩[n..] ≅ hf'⟨wk_up ℓf ρ⟩[n'..] : P⟨wk_up ℓ ρ⟩[(tBox ℓ (tEval ℓf n))..] | RPP'extf Δ ρ wfΔ _ _ Rn]).
+(*     (Rht : [Γ,,ℓt ||-< l > ht ≅ ht' : _ |RPP't])
+    (Rhf : [Γ,,ℓf ||-< l > hf ≅ hf' : _ |RPP'f]). *)
+
+  Let RPext : forall Δ (ρ : Δ ≤ Γ) (wfΔ : [|-Δ]), forall n n', [Δ ||-EllS n ≅ n' : ℓ | SNtoBRedEqTy (l:=l) wfΔ] ->
+      [Δ ||-< l > P⟨wk_up ℓ ρ⟩[n..] ≅ P⟨wk_up ℓ ρ⟩[n'..]].
+  Proof.
+    intros * Rn0.
+    etransitivity; [|symmetry]; eapply RPP'ext.
+    1: eapply Rn0.
+    eapply urefl; tea.
+  Qed.
+
+  Let RPP'tt := RPP'extt _ (wk1 ℓt) wfΓℓt _ _ (Svar0Ell _).
+  Let Rht : [Γ,,ℓt ||-< l > ht ≅ ht' : _|RPP'tt].
+  Proof.
+    specialize (Rhtext _ (wk1 ℓt) wfΓℓt _ _ (Svar0Ell _)) as Rht.
+    now rewrite ! wk1_eta in Rht.
+  Qed.
+  Let RPP'ff := RPP'extf _ (wk1 ℓf) wfΓℓf _ _ (Svar0Ell _).
+  Let Rhf : [Γ,,ℓf ||-< l > hf ≅ hf' : _|RPP'ff].
+  Proof.
+    specialize (Rhfext _ (wk1 ℓf) wfΓℓf _ _ (Svar0Ell _)) as Rhf.
+    now rewrite ! wk1_eta in Rhf.
+  Qed.
+
+  Lemma SEllElimRedEqAux : forall b b' (Rbb' : BoolPropEq Γ b b')
+    (Rnb : [Γ ||-S< l > tApp (tEval ℓ t) (nat_to_term k) ≅ b : tBool | RB])
+    (Rn'b : [Γ ||-S< l > tApp (tEval ℓ t') (nat_to_term k) ≅ b : tBool | RB]),
+    [Γ ||-< l > tEllElim k ℓ P ht hf t b ≅ tEllElim k ℓ P' ht' hf' t' b' : P[t..] | RPP't].
+  Proof.
+    clear dependent b. clear b'.
+    intros ?? propbb' Rnb Rn'b.
+    destruct propbb'.
+    - escape.
+      eapply redSubstTmEq.
+      2: eapply redtm_ellElimTrue; tea.
+      2:{ eapply redtm_ellElimTrue; tea.
+        1,2 : eapply ty_conv; tea. }
+      rewrite <- (wk_id_ren_on (Γ,,ℓt) ht), <- (wk_id_ren_on (Γ,,ℓt) ht'),
+        <-2 wk_up_wk_id.
+      assert (Rtnbt : forall n b, in_ell ℓt n b ->
+        [Γ ||-S< l > tApp (tEval ℓ t) (nat_to_term n) ≅ bool_to_term b : _ | SboolRed wfΓ]).
+      { intros n b [[-> ->]| [inℓ]]%in_cons_ell_relevant; tea.
+        eapply evalnat_to_termRed; tea. }
+      assert (Rt'nbt : forall n b, in_ell ℓt n b ->
+        [Γ ||-S< l > tApp (tEval ℓ t') (nat_to_term n) ≅ bool_to_term b : _ | SboolRed wfΓ]).
+      { intros n b [[-> ->]| [inℓ]]%in_cons_ell_relevant; tea.
+        eapply evalnat_to_termRed; tea; symmetry; tea. }
+      assert (Rboxeval : [Γ ||-EllS tBox ℓt (tEval ℓ t) ≅ tBox ℓt (tEval ℓ t'): ℓt | SNtoBRedEqTy (l:=l) wfΓ]).
+      { eapply SboxRed; tea.
+        eapply Rt. }
+      unshelve eapply irrLRConv, Rhtext; tea.
+      replace P[t..] with P⟨wk_up ℓ (@wk_id Γ)⟩[t..] by
+        now rewrite wk_up_wk_id, wk_id_ren_on.
+      unshelve eapply RPext; tea.
+      etransitivity.
+      + eapply SboxRed; tea.
+        { eapply evalBoxRed, lrefl, Rt; tea. }
+        * intros n b inℓ.
+          eapply evalnat_to_termRed; tea.
+          eapply in_cons_ell; right; tea.
+        * intros n b inℓ.
+          eapply evalnat_to_termRed; tea.
+      + now eapply etaEllRed, lrefl.
+    - escape.
+      eapply redSubstTmEq.
+      2: eapply redtm_ellElimFalse; tea.
+      2:{ eapply redtm_ellElimFalse; tea.
+        1,2 : eapply ty_conv; tea. }
+      rewrite <- (wk_id_ren_on (Γ,,ℓf) hf), <- (wk_id_ren_on (Γ,,ℓf) hf'),
+        <-2 wk_up_wk_id.
+      assert (Rtnbf : forall n b, in_ell ℓf n b ->
+        [Γ ||-S< l > tApp (tEval ℓ t) (nat_to_term n) ≅ bool_to_term b : _ | SboolRed wfΓ]).
+      { intros n b [[-> ->]| [inℓ]]%in_cons_ell_relevant; tea.
+        eapply evalnat_to_termRed; tea. }
+      assert (Rt'nbf : forall n b, in_ell ℓf n b ->
+        [Γ ||-S< l > tApp (tEval ℓ t') (nat_to_term n) ≅ bool_to_term b : _ | SboolRed wfΓ]).
+      { intros n b [[-> ->]| [inℓ]]%in_cons_ell_relevant; tea.
+        eapply evalnat_to_termRed; tea; symmetry; tea. }
+      assert (Rboxeval : [Γ ||-EllS tBox ℓf (tEval ℓ t) ≅ tBox ℓf (tEval ℓ t'): ℓf | SNtoBRedEqTy (l:=l) wfΓ]).
+      { eapply SboxRed; tea.
+        eapply Rt. }
+      unshelve eapply irrLRConv, Rhfext; tea.
+      replace P[t..] with P⟨wk_up ℓ (@wk_id Γ)⟩[t..] by
+        now rewrite wk_up_wk_id, wk_id_ren_on.
+      unshelve eapply RPext; tea.
+      etransitivity.
+      + eapply SboxRed; tea.
+        { eapply evalBoxRed, lrefl, Rt; tea. }
+        * intros n b inℓ.
+          eapply evalnat_to_termRed; tea.
+          eapply in_cons_ell; right; tea.
+        * intros n b inℓ.
+          eapply evalnat_to_termRed; tea.
+      + now eapply etaEllRed, lrefl.
+  - epose proof (SneNfTermEq RB r).
+    escape.
+    eapply irrLR, neNfTermEq; constructor.
+    + eapply ty_ellElim; tea.
+    + eapply ty_conv.
+      { eapply ty_ellElim; tea.
+        - eapply ty_conv; tea.
+        - eapply ty_conv; tea.
+        - etransitivity; tea. }
+      now symmetry.
+    + destruct r; eapply convneu_ellElim; tea.
+  Unshelve.
+  tea.
+  eapply lrefl; tea.
+  Qed.
+
+  Lemma SEllElimRedEq :
+    [Γ ||-< l > tEllElim k ℓ P ht hf t b ≅ tEllElim k ℓ P' ht' hf' t' b' : P[t..] | RPP't].
+  Proof.
+    destruct Rb as [?? [] []].
+    escape.
+    eapply redSubstTmEq.
+    2,3: eapply redtm_ellElim; tea.
+    2,3: eapply ty_conv; tea.
+    2: etransitivity; tea.
+    eapply SEllElimRedEqAux; tea.
+    1,2: etransitivity; tea.
+    1,2: eapply SredSubstLeftTmEq; tea; eapply lrefl; tea;
+      eexists nfL nfR; tea; eapply redtmwf_refl; tea.
+  Qed.
+End SEllElimRedEq.
+
+  Section EllElimRedEq.
+  Context {Γ l ℓ k P P' t t' b b'} (wfΓ : [|-Γ]) (ℓt := cons_ell ℓ k true) (ℓf := cons_ell ℓ k false)
+    (RB := boolRed (l:=l) wfΓ) (RN := natRed (l:=l) wfΓ)
+    (RNtoB := NtoBRedEqTy (l:=l) wfΓ)
+    (gP : [Γ,,ℓ |- P]) (gP' : [Γ,,ℓ |- P']) (gPP' : [Γ,,ℓ |- P ≅ P'])
+    (RPP'ext : forall Δ (ρ : Δ ≤ Γ) (wfΔ : [|-Δ]), forall t t', [Δ ||-Ell t ≅ t' : ℓ | NtoBRedEqTy (l:=l) wfΔ] ->
+      [Δ ||-< l > P⟨wk_up ℓ ρ⟩[t..] ≅ P'⟨wk_up ℓ ρ⟩[t'..]])
+    (Rt  : [Γ ||-Ell t ≅ t' : ℓ | RNtoB]) (Rb : [Γ ||-< l > b ≅ b' : tBool | RB])
+    (Rtkb : [Γ ||-< l > tApp (tEval ℓ t) (nat_to_term k) ≅ b : tBool | RB])
+    (Rt'kb : [Γ ||-< l > tApp (tEval ℓ t') (nat_to_term k) ≅ b : tBool | RB])
+    (Pt := P⟨wk_up ℓ (@wk1 Γ ℓt)⟩[(tBox ℓ (tEval ℓt (tRel 0)))..])
+    (Pf := P⟨wk_up ℓ (@wk1 Γ ℓf)⟩[(tBox ℓ (tEval ℓf (tRel 0)))..])
+    (P't := P'⟨wk_up ℓ (@wk1 Γ ℓt)⟩[(tBox ℓ (tEval ℓt (tRel 0)))..])
+    (P'f := P'⟨wk_up ℓ (@wk1 Γ ℓf)⟩[(tBox ℓ (tEval ℓf (tRel 0)))..])
+    (wfΓℓ := wfc_consell (ℓ:=ℓ) wfΓ)
+    (wfΓℓt := wfc_consell (ℓ:=ℓt) wfΓ)
+    (wfΓℓf := wfc_consell (ℓ:=ℓf) wfΓ).
+  Let RPP' : [Γ,,ℓ ||-< l > P ≅ P'].
+  Proof.
+    rewrite <- (wk1_eta (Γ:=Γ) (A:=ℓ) (t:=P)), <- (wk1_eta (Γ:=Γ) (A:=ℓ) (t:=P')).
+    unshelve eapply RPP'ext; tea.
+    eapply reflectEll.
+    repeat constructor.
+  Qed.
+  Let RPP'extt : forall Δ (ρ : Δ ≤ Γ) (wfΔ : [|-Δ]), forall n n', [Δ ||-Ell n ≅ n' : ℓt | NtoBRedEqTy (l:=l) wfΔ] ->
+      [Δ ||-< l > P⟨wk_up ℓ ρ⟩[(tBox ℓ (tEval ℓt n))..] ≅ P'⟨wk_up ℓ ρ⟩[(tBox ℓ (tEval ℓt n'))..]].
+  Proof.
+    intros * Rn0.
+    unshelve eapply RPP'ext; tea.
+    eapply boxRed.
+    + eapply EvalRedEq; tea.
+    + intros ?? inℓ.
+      eapply evalnat_to_termRed; tea.
+      eapply in_cons_ell; right; tea.
+    + intros ?? inℓ.
+      eapply evalnat_to_termRed, PER_Symmetric; tea.
+      eapply in_cons_ell; right; tea.
+  Qed.
+  Let RPP'extf : forall Δ (ρ : Δ ≤ Γ) (wfΔ : [|-Δ]), forall n n', [Δ ||-EllS n ≅ n' : ℓf | SNtoBRedEqTy (l:=l) wfΔ] ->
+      [Δ ||-< l > P⟨wk_up ℓ ρ⟩[(tBox ℓ (tEval ℓf n))..] ≅ P'⟨wk_up ℓ ρ⟩[(tBox ℓ (tEval ℓf n'))..]].
+  Proof.
+    intros * Rn0.
+    unshelve eapply RPP'ext; tea.
+    eapply SboxRed.
+    + eapply EvalRedEq; tea.
+    + intros ?? inℓ.
+      eapply evalnat_to_termRed; tea.
+      eapply in_cons_ell; right; tea.
+    + intros ?? inℓ.
+      eapply evalnat_to_termRed, PER_Symmetric; tea.
+      eapply in_cons_ell; right; tea.
+  Qed.
+
+  Let RPP't : [Γ ||-< l > P[t..] ≅ P'[t'..]].
+  Proof.
+    rewrite <- (wk_id_ren_on (Γ,,ℓ) P), <- (wk_id_ren_on (Γ,,ℓ) P'),
+      <- 2 wk_up_wk_id.
+    unshelve eapply RPP'ext; tea.
+  Qed.
+  Context {ht ht' hf hf'}
+    (Rhtext : forall Δ (ρ : Δ ≤ Γ) (wfΔ : [|-Δ]), forall n n' (Rn : [Δ ||-EllS n ≅ n' : ℓt | SNtoBRedEqTy (l:=l) wfΔ]),
+      [Δ ||-< l > ht⟨wk_up ℓt ρ⟩[n..] ≅ ht'⟨wk_up ℓt ρ⟩[n'..] : P⟨wk_up ℓ ρ⟩[(tBox ℓ (tEval ℓt n))..] | RPP'extt Δ ρ wfΔ _ _ Rn])
+    (Rhfext : forall Δ (ρ : Δ ≤ Γ) (wfΔ : [|-Δ]), forall n n' (Rn : [Δ ||-EllS n ≅ n' : ℓf | SNtoBRedEqTy (l:=l) wfΔ]),
+      [Δ ||-< l > hf⟨wk_up ℓf ρ⟩[n..] ≅ hf'⟨wk_up ℓf ρ⟩[n'..] : P⟨wk_up ℓ ρ⟩[(tBox ℓ (tEval ℓf n))..] | RPP'extf Δ ρ wfΔ _ _ Rn]).
+(*     (Rht : [Γ,,ℓt ||-< l > ht ≅ ht' : _ |RPP't])
+    (Rhf : [Γ,,ℓf ||-< l > hf ≅ hf' : _ |RPP'f]). *)
+
+  Let RPext : forall Δ (ρ : Δ ≤ Γ) (wfΔ : [|-Δ]), forall n n', [Δ ||-EllS n ≅ n' : ℓ | SNtoBRedEqTy (l:=l) wfΔ] ->
+      [Δ ||-< l > P⟨wk_up ℓ ρ⟩[n..] ≅ P⟨wk_up ℓ ρ⟩[n'..]].
+  Proof.
+    intros * Rn0.
+    etransitivity; [|symmetry]; eapply RPP'ext.
+    1: eapply Rn0.
+    eapply urefl; tea.
+  Qed.
+
+  Let RPP'tt := RPP'extt _ (wk1 ℓt) wfΓℓt _ _ (Svar0Ell _).
+  Let Rht : [Γ,,ℓt ||-< l > ht ≅ ht' : _|RPP'tt].
+  Proof.
+    specialize (Rhtext _ (wk1 ℓt) wfΓℓt _ _ (Svar0Ell _)) as Rht.
+    now rewrite ! wk1_eta in Rht.
+  Qed.
+  Let RPP'ff := RPP'extf _ (wk1 ℓf) wfΓℓf _ _ (Svar0Ell _).
+  Let Rhf : [Γ,,ℓf ||-< l > hf ≅ hf' : _|RPP'ff].
+  Proof.
+    specialize (Rhfext _ (wk1 ℓf) wfΓℓf _ _ (Svar0Ell _)) as Rhf.
+    now rewrite ! wk1_eta in Rhf.
+  Qed.
+
+  Lemma SEllElimRedEqAux : forall b b' (Rbb' : BoolPropEq Γ b b')
+    (Rnb : [Γ ||-S< l > tApp (tEval ℓ t) (nat_to_term k) ≅ b : tBool | RB])
+    (Rn'b : [Γ ||-S< l > tApp (tEval ℓ t') (nat_to_term k) ≅ b : tBool | RB]),
+    [Γ ||-< l > tEllElim k ℓ P ht hf t b ≅ tEllElim k ℓ P' ht' hf' t' b' : P[t..] | RPP't].
+  Proof.
+    clear dependent b. clear b'.
+    intros ?? propbb' Rnb Rn'b.
+    destruct propbb'.
+    - escape.
+      eapply redSubstTmEq.
+      2: eapply redtm_ellElimTrue; tea.
+      2:{ eapply redtm_ellElimTrue; tea.
+        1,2 : eapply ty_conv; tea. }
+      rewrite <- (wk_id_ren_on (Γ,,ℓt) ht), <- (wk_id_ren_on (Γ,,ℓt) ht'),
+        <-2 wk_up_wk_id.
+      assert (Rtnbt : forall n b, in_ell ℓt n b ->
+        [Γ ||-S< l > tApp (tEval ℓ t) (nat_to_term n) ≅ bool_to_term b : _ | SboolRed wfΓ]).
+      { intros n b [[-> ->]| [inℓ]]%in_cons_ell_relevant; tea.
+        eapply evalnat_to_termRed; tea. }
+      assert (Rt'nbt : forall n b, in_ell ℓt n b ->
+        [Γ ||-S< l > tApp (tEval ℓ t') (nat_to_term n) ≅ bool_to_term b : _ | SboolRed wfΓ]).
+      { intros n b [[-> ->]| [inℓ]]%in_cons_ell_relevant; tea.
+        eapply evalnat_to_termRed; tea; symmetry; tea. }
+      assert (Rboxeval : [Γ ||-EllS tBox ℓt (tEval ℓ t) ≅ tBox ℓt (tEval ℓ t'): ℓt | SNtoBRedEqTy (l:=l) wfΓ]).
+      { eapply SboxRed; tea.
+        eapply Rt. }
+      unshelve eapply irrLRConv, Rhtext; tea.
+      replace P[t..] with P⟨wk_up ℓ (@wk_id Γ)⟩[t..] by
+        now rewrite wk_up_wk_id, wk_id_ren_on.
+      unshelve eapply RPext; tea.
+      etransitivity.
+      + eapply SboxRed; tea.
+        { eapply evalBoxRed, lrefl, Rt; tea. }
+        * intros n b inℓ.
+          eapply evalnat_to_termRed; tea.
+          eapply in_cons_ell; right; tea.
+        * intros n b inℓ.
+          eapply evalnat_to_termRed; tea.
+      + now eapply etaEllRed, lrefl.
+    - escape.
+      eapply redSubstTmEq.
+      2: eapply redtm_ellElimFalse; tea.
+      2:{ eapply redtm_ellElimFalse; tea.
+        1,2 : eapply ty_conv; tea. }
+      rewrite <- (wk_id_ren_on (Γ,,ℓf) hf), <- (wk_id_ren_on (Γ,,ℓf) hf'),
+        <-2 wk_up_wk_id.
+      assert (Rtnbf : forall n b, in_ell ℓf n b ->
+        [Γ ||-S< l > tApp (tEval ℓ t) (nat_to_term n) ≅ bool_to_term b : _ | SboolRed wfΓ]).
+      { intros n b [[-> ->]| [inℓ]]%in_cons_ell_relevant; tea.
+        eapply evalnat_to_termRed; tea. }
+      assert (Rt'nbf : forall n b, in_ell ℓf n b ->
+        [Γ ||-S< l > tApp (tEval ℓ t') (nat_to_term n) ≅ bool_to_term b : _ | SboolRed wfΓ]).
+      { intros n b [[-> ->]| [inℓ]]%in_cons_ell_relevant; tea.
+        eapply evalnat_to_termRed; tea; symmetry; tea. }
+      assert (Rboxeval : [Γ ||-EllS tBox ℓf (tEval ℓ t) ≅ tBox ℓf (tEval ℓ t'): ℓf | SNtoBRedEqTy (l:=l) wfΓ]).
+      { eapply SboxRed; tea.
+        eapply Rt. }
+      unshelve eapply irrLRConv, Rhfext; tea.
+      replace P[t..] with P⟨wk_up ℓ (@wk_id Γ)⟩[t..] by
+        now rewrite wk_up_wk_id, wk_id_ren_on.
+      unshelve eapply RPext; tea.
+      etransitivity.
+      + eapply SboxRed; tea.
+        { eapply evalBoxRed, lrefl, Rt; tea. }
+        * intros n b inℓ.
+          eapply evalnat_to_termRed; tea.
+          eapply in_cons_ell; right; tea.
+        * intros n b inℓ.
+          eapply evalnat_to_termRed; tea.
+      + now eapply etaEllRed, lrefl.
+  - epose proof (SneNfTermEq RB r).
+    escape.
+    eapply irrLR, neNfTermEq; constructor.
+    + eapply ty_ellElim; tea.
+    + eapply ty_conv.
+      { eapply ty_ellElim; tea.
+        - eapply ty_conv; tea.
+        - eapply ty_conv; tea.
+        - etransitivity; tea. }
+      now symmetry.
+    + destruct r; eapply convneu_ellElim; tea.
+  Unshelve.
+  tea.
+  eapply lrefl; tea.
+  Qed.
+
+  Lemma SEllElimRedEq :
+    [Γ ||-< l > tEllElim k ℓ P ht hf t b ≅ tEllElim k ℓ P' ht' hf' t' b' : P[t..] | RPP't].
+  Proof.
+    destruct Rb as [?? [] []].
+    escape.
+    eapply redSubstTmEq.
+    2,3: eapply redtm_ellElim; tea.
+    2,3: eapply ty_conv; tea.
+    2: etransitivity; tea.
+    eapply SEllElimRedEqAux; tea.
+    1,2: etransitivity; tea.
+    1,2: eapply SredSubstLeftTmEq; tea; eapply lrefl; tea;
+      eexists nfL nfR; tea; eapply redtmwf_refl; tea.
+  Qed.
+End SEllElimRedEq.
+End Ell.
 End Ell.
